src/lang.v
@@ -27,7 +27,7 @@ Definition place : Set := var * path.
 
 Inductive type :=
 | TInt
-| TRef (t : type)
+| TRef
 | TPair (t1 t2 : type)
 .
 
@@ -57,10 +57,10 @@ Notation "'INT' p" := (IntConst TInt p) (at level 80, p at next level).
 Notation "'ASSIGN' p <- rv" := (Assign p rv) (at level 90).
 
 Local Open Scope positive_scope.
-Check (&mut (1, nil) : TRef TInt) : rvalue.
-Check (ASSIGN (2, nil) <- &mut (1, nil) : TRef TInt).
+Check (&mut (1, nil) : TRef) : rvalue.
+Check (ASSIGN (2, nil) <- &mut (1, nil) : TRef).
 Check (ASSIGN (1, nil) <- Just TInt (INT 3)).
-Check (ASSIGN (1, nil) <- Just TInt (INT 3) ;; ((ASSIGN (2, nil) <- &mut (1, nil) : TRef TInt) ;; Panic)).
+Check (ASSIGN (1, nil) <- Just TInt (INT 3) ;; ((ASSIGN (2, nil) <- &mut (1, nil) : TRef ) ;; Panic)).
 
 (* These definitions are not part of the grammar, but they are common for several (all?) semantics of the LLBC. *)
 Definition loan_id := nat.
